Value restriction.

theories/case_studies/c.v
@@ -30,8 +30,7 @@ Opaque sem_ty_void sem_ty_unit sem_ty_bool sem_ty_int sem_ty_string sem_ty_top s
 Opaque sem_sig_eff sem_sig_flip_bang.
 Opaque sem_row_nil sem_row_flip_bang sem_row_cons sem_row_rec.
 
-Definition C : val := (Λ: Λ: Λ: Λ: λ: "x" "y" "z", ("x" "z") "y")%V.
-Definition C_gen : val := (Λ: C)%V.
+Definition C : val := (λ: "x" "y" "z", ("x" "z") "y")%V.
 
 Section typing.
 
@@ -50,14 +49,10 @@ Section typing.
   Proof.
     iIntros. rewrite /C /C_os_ty.
     iApply sem_typed_Rclosure; solve_sidecond. iIntros (θ).
-    rewrite - (app_nil_l []).
-    iApply sem_typed_TLam; solve_sidecond. iIntros (α).
-    rewrite - (app_nil_l []).
-    iApply sem_typed_TLam; solve_sidecond. iIntros (β).
-    rewrite - (app_nil_l []).
-    iApply sem_typed_TLam; solve_sidecond. iIntros (γ).
-    rewrite - (app_nil_l []).
-    iApply sem_typed_ufun; solve_sidecond. simpl.
+    iApply sem_typed_Tclosure; solve_sidecond. iIntros (α).
+    iApply sem_typed_Tclosure; solve_sidecond. iIntros (β).
+    iApply sem_typed_Tclosure; solve_sidecond. iIntros (γ).
+    iApply sem_typed_closure; solve_sidecond. simpl.
     rewrite - (app_nil_r [("x", _)]).
     iApply sem_typed_afun; solve_sidecond. simpl.
     rewrite - (app_nil_r [("y", _); ("x", _)]).
@@ -72,14 +67,10 @@ Section typing.
   Proof.
     iIntros. rewrite /C /C_ms_ty.
     iApply sem_typed_Rclosure; solve_sidecond. iIntros (θ).
-    rewrite - (app_nil_l []).
-    iApply sem_typed_TLam; solve_sidecond. iIntros (α).
-    rewrite - (app_nil_l []).
-    iApply sem_typed_TLam; solve_sidecond. iIntros (β).
-    rewrite - (app_nil_l []).
-    iApply sem_typed_TLam; solve_sidecond. iIntros (γ).
-    rewrite - (app_nil_l []).
-    iApply sem_typed_ufun; solve_sidecond. simpl.
+    iApply sem_typed_Tclosure; solve_sidecond. iIntros (α).
+    iApply sem_typed_Tclosure; solve_sidecond. iIntros (β).
+    iApply sem_typed_Tclosure; solve_sidecond. iIntros (γ).
+    iApply sem_typed_closure; solve_sidecond. simpl.
     rewrite - (app_nil_r [("x", _)]).
     iApply sem_typed_afun; solve_sidecond. simpl.
     rewrite - (app_nil_r [("y", _); ("x", _)]).
@@ -90,27 +81,15 @@ Section typing.
     iApply sem_typed_var'.
   Qed.
 
-  Lemma C_gen_typed_alt : ⊢ ⊨ᵥ C_gen : C_gen_ty.
+  Lemma C_gen_typed : ⊢ ⊨ᵥ C : C_gen_ty.
   Proof.
-    iIntros. rewrite /C_gen /C_gen_ty /C.
-    iApply sem_typed_Mclosure_alt.
-    { iApply sem_typed_val. iApply C_os_typed. }
-    iApply sem_typed_val. iApply C_ms_typed.
-  Qed.
-
-  Lemma C_gen_typed : ⊢ ⊨ᵥ C_gen : C_gen_ty.
-  Proof.
-    iIntros. rewrite /C_gen /C_gen_ty /C.
+    iIntros. rewrite /C_gen_ty /C.
     iApply sem_typed_Mclosure; solve_sidecond. iIntros (ν).
-    iApply sem_typed_val. iApply sem_typed_Rclosure; solve_sidecond. iIntros (θ).
-    rewrite - (app_nil_l []).
-    iApply sem_typed_TLam; solve_sidecond. iIntros (α).
-    rewrite - (app_nil_l []).
-    iApply sem_typed_TLam; solve_sidecond. iIntros (β).
-    rewrite - (app_nil_l []).
-    iApply sem_typed_TLam; solve_sidecond. iIntros (γ).
-    rewrite - (app_nil_l []).
-    iApply sem_typed_ufun; solve_sidecond. simpl.
+    iApply sem_typed_Rclosure; solve_sidecond. iIntros (θ).
+    iApply sem_typed_Tclosure; solve_sidecond. iIntros (α).
+    iApply sem_typed_Tclosure; solve_sidecond. iIntros (β).
+    iApply sem_typed_Tclosure; solve_sidecond. iIntros (γ).
+    iApply sem_typed_closure; solve_sidecond. simpl.
     rewrite - (app_nil_r [("x", _)]).
     iApply sem_typed_afun; solve_sidecond. simpl.
     rewrite - (app_nil_r [("y", _); ("x", _)]).
