install.sh
@@ -3,8 +3,8 @@ echo "...Affect Setup..."
 
 export OPAMYES=true
 
-echo "∙ Creating new opam switch"
-opam switch create affect ocaml-base-compiler.5.0.0
+#echo "∙ Creating new opam switch"
+#opam switch create affect ocaml-base-compiler.5.0.0
 
 echo "∙ Fetching coq-hazel library"
 git clone https://gitlab.inria.fr/cambium/hazel
@@ -19,12 +19,12 @@ git apply ../hazel.patch
 echo "∙ Commiting patch"
 git add .; git commit -m "Hazel patch for Affect applied" 
 
-echo "∙ Installing coq-hazel"
-opam install . 
-cd ..
+#echo "∙ Installing coq-hazel"
+#opam install . 
+#cd ..
 
-echo "∙ Installing local dependencies"
-opam install . --deps-only
+#echo "∙ Installing local dependencies"
+#opam install . --deps-only
 
-echo "∙ Compiling Affect"
-make
+#echo "∙ Compiling Affect"
+#make
